Rustv/Tests/ex/Swap_CounterExample.thy
@@ -1,0 +1,176 @@
+theory Swap_CounterExample
+  imports Simpl.Semantic Simpl.Vcg "Rust-Verification.Rust_Semantics"
+begin
+
+record rustv_swap_env = globals_ram +
+  x :: tagged_ref
+  y :: tagged_ref
+  tmp :: tagged_ref
+
+definition rustv_swap_body :: "(rustv_swap_env, 'p, rust_error) com" where
+  "rustv_swap_body ==
+    Basic (\<lambda>s. let (r, s') = heap_new uninit s in s'\<lparr> tmp := r \<rparr>);;
+    copy_betw_places x tmp;;
+    copy_betw_places y x;;
+    copy_betw_places tmp y"
+
+definition root where
+  "root = tag_val 0"
+definition s1 where
+  "s1 = tag_val 1"
+definition u where
+  "u = tag_val 2"
+definition s2 where
+  "s2 = tag_val 3"
+definition borrow_stack where
+  "borrow_stack = [(SharedReadWrite, {s2}), (Unique, {u}),
+    (SharedReadWrite, {s1}), (Unique, {root})]"
+
+lemma l1: "wf_reborrow borrow_stack"
+  unfolding borrow_stack_def
+  apply (rule ReborrowUniqueSRW)
+   apply (rule ReborrowSRWUnique)
+    apply (rule ReborrowUniqueSRW)
+     apply (rule BorrowRoot)
+  by (simp_all add: root_def s1_def u_def s2_def)
+
+definition the_memory :: rustv_swap_env where
+  "the_memory = \<lparr>
+    memory = [int_val 100],
+    tags = [borrow_stack],
+    issued_tags = [root, s1, u, s2],
+    x = \<lparr> pointer = ptr_val 0, tag = s1 \<rparr>,
+    y = \<lparr> pointer = ptr_val 0, tag = s2 \<rparr>,
+    tmp = undefined
+  \<rparr>"
+
+lemma l2: "wf_heap the_memory"
+  apply (auto simp add: the_memory_def borrow_stack_def)
+  using l1 by (simp add: borrow_stack_def)
+
+lemma l3: "(let (r, s') = heap_new uninit the_memory
+     in s'\<lparr>tmp := r\<rparr>)
+    \<in> {s. Rustv.writable (tmp s) s \<and>
+           Rustv.readable (x s) s}"
+  unfolding the_memory_def
+  by (auto simp add: Let_def borrow_stack_def)
+
+lemma l4: "\<Gamma> \<turnstile>\<langle>rustv_swap_body, Normal the_memory\<rangle> \<Rightarrow> Fault invalid_ref"
+  unfolding rustv_swap_body_def
+  apply (rule Semantic.exec.Seq)
+   apply (rule Semantic.exec.Seq)
+    apply (rule Semantic.exec.Seq)
+     apply (rule Semantic.exec.Basic)
+    apply (rule Semantic.exec.Guard)
+     apply (rule l3)
+    apply (rule Semantic.exec.Seq)
+     apply (rule Semantic.exec.Seq)
+      apply (rule Semantic.exec.Basic)
+     apply (rule Semantic.exec.Basic)
+    apply (rule Semantic.exec.Basic)
+   apply (rule Semantic.exec.GuardFault)
+   prefer 2
+   apply simp
+  by (auto simp add: Let_def the_memory_def borrow_stack_def s1_def s2_def u_def root_def)
+
+lemma l6: "writable (x the_memory) the_memory"
+  unfolding the_memory_def borrow_stack_def
+  by simp
+
+lemma l7: "writable (y the_memory) the_memory"
+  unfolding the_memory_def borrow_stack_def
+  by simp
+
+theorem "\<exists>s.
+  writable (x s) s \<and>
+  writable (y s) s \<and>
+  \<Gamma> \<turnstile> \<langle>rustv_swap_body, Normal s\<rangle> \<Rightarrow> Fault invalid_ref"
+  using l4 l6 l7 by auto
+
+inductive det where
+  DetBasic: "det (Basic f)" |
+  DetSeq: "\<lbrakk>det c1; det c2\<rbrakk> \<Longrightarrow> det (c1;; c2)" |
+  DetGuard: "det c \<Longrightarrow> det (Guard f g c)"
+
+lemma det_det:
+  assumes
+    "det c"
+    "\<Gamma> \<turnstile> \<langle>c, s\<rangle> \<Rightarrow> t"
+    "\<Gamma> \<turnstile> \<langle>c, s\<rangle> \<Rightarrow> t'"
+  shows "t = t'"
+using assms proof (induction arbitrary: s t t')
+  case (DetBasic f)
+  then show ?case
+    by (metis exec_Normal_elim_cases(6) exec_elim_cases(7))
+next
+  case (DetSeq c1 c2)
+  show ?case
+  proof (cases s)
+    case (Normal x1)
+    then show ?thesis
+      by (metis DetSeq.IH DetSeq.prems exec_Normal_elim_cases(8))
+  next
+    case (Abrupt x2)
+    then show ?thesis
+      by (metis Abrupt_end DetSeq.prems(1) DetSeq.prems(2))
+  next
+    case (Fault x3)
+    then show ?thesis
+      by (metis Fault_end DetSeq.prems(1) DetSeq.prems(2))
+  next
+    case Stuck
+    then show ?thesis
+      by (metis Stuck_end DetSeq.prems(1) DetSeq.prems(2))
+  qed
+next
+  case (DetGuard c f g)
+  thm exec_Normal_elim_cases(5)
+  thm exec_elim_cases
+  show ?case
+  proof (cases s)
+    case (Normal x1)
+    then show ?thesis
+      by (metis DetGuard.IH DetGuard.prems exec_Normal_elim_cases(5))
+  next
+    case (Abrupt x2)
+    then show ?thesis
+      by (metis Abrupt_end DetGuard.prems(1) DetGuard.prems(2))
+  next
+    case (Fault x3)
+    then show ?thesis
+      by (metis Fault_end DetGuard.prems(1) DetGuard.prems(2))
+  next
+    case Stuck
+    then show ?thesis
+      by (metis Stuck_end DetGuard.prems(1) DetGuard.prems(2))
+  qed
+qed
+
+lemma det_swap: "det rustv_swap_body"
+  unfolding rustv_swap_body_def
+  by (simp add: DetBasic DetGuard DetSeq)
+
+lemma l5: "\<Gamma> \<turnstile>\<langle>rustv_swap_body, Normal the_memory\<rangle> \<Rightarrow> t \<Longrightarrow> t = Fault invalid_ref"
+proof -
+  assume "\<Gamma> \<turnstile>\<langle>rustv_swap_body, Normal the_memory\<rangle> \<Rightarrow> t"
+  then show "t = Fault invalid_ref"
+    using det_det det_swap l4 by blast
+qed
+
+theorem "\<exists>s.
+  writable (x s) s \<and>
+  writable (y s) s \<and>
+  (\<forall>t. \<Gamma> \<turnstile> \<langle>rustv_swap_body, Normal s\<rangle> \<Rightarrow> t \<longrightarrow> t = Fault invalid_ref)"
+  using l5 l6 l7 by auto
+
+lemma "\<Gamma> \<turnstile>\<^bsub>/{invalid_ref}\<^esub>
+  {s. s = the_memory}
+  rustv_swap_body
+  {s. False}, {s. False}"
+  unfolding rustv_swap_body_def
+  apply vcg
+  apply (auto simp add: Let_def)
+  by (auto simp add: the_memory_def borrow_stack_def
+      s1_def s2_def u_def root_def)
+
+end
